\documentclass{article}
\usepackage[utf8]{inputenc}
\usepackage{amsmath}
\usepackage{geometry}
\geometry{margin=1in}

\title{\vspace{-5.5cm}Random Graphs Project 1}
\author{Alex Rose, Pedro}
\date{February 2016}

\begin{document}

\maketitle

\section{Warm-Up Identities}

\subsection{}
$$ C'(z) =\sum_{n \ge 0} \frac{c_n}{n!} * \frac{d}{dz} z^n = \sum_{n \ge 1} \frac{c_n}{n!}nz^{n-1}$$ 
$$\newline = \sum_{n \ge 1} \frac{c_n}{(n-1)!}z^{n-1} = \sum_{n \ge 0} \frac{c_{n+1}}{n!}z^{n} = (c_{n+1})_{n \ge 0} $$

\subsection{}
$$ \int_{0}^{z} C(t) dt  =\sum_{n \ge 0} \frac{c_n}{n!} * \int_{0}^{z} t^n dt = \sum_{n \ge 1} \frac{c_n}{n!} \frac{z^{n+1}}{n+1}$$ 
$$\newline = \sum_{n \ge 0} \frac{c_n}{(n+1)!}z^{n+11} = \sum_{n \ge 1} \frac{c_{n-1}}{n!}z^{n} = (c_{n-1})_{n \ge 1} $$ 

\section{Pointed Class}
For each object of size n, we have n ways of choosing the pointer, one for each element in the object. So the pointed class generating function is of the form:

$$C^\swarrow(z) = \sum_{n \ge 0} n\frac{c_n}{n!}z^n = \sum_{n \ge 0} \frac{c_n}{(n-1)!}zz^{n-1} = z\sum_{n \ge 0} \frac{c_n}{(n-1)!}z^{n-1} = z\sum_{n \ge 0} \frac{c_{n+1}}{n!}z^{n}$$

And from (1.1), the remaining sum is equal to $C'(z)$. So $C^\swarrow(z) = zC'(z)$.


\section{Modified Labelled Product}

\subsection{}
The recursion for the \textit{unlabelled} $c_n$, in terms of $a_n$ and $b_n$, is given by:

$$c_n = \sum_{i + k = n} a_ib_k$$

As a particular index must be in A, we choose $k$ labels from a pool of $n-1 = i + k - 1$ labels for the B-member. Thus our labelled recursion is of the form:

$$c_n = \sum_{i + k = n} \binom{i + k - 1}{k}a_ib_k$$

\subsection{}

Note that:

$$C(z) =  \int_{0}^{z} C'(t) dt = \int_{0}^{z} \sum_{n \ge 0} \frac{c_{n+1}}{n!}t^{n}  = \int_{0}^{z} \sum_{n \ge 1} \frac{c_n}{(n-1)!}t^{n-1}  dt$$ 

We seek the value of the inner sum, $C'(z)$. Substituting $c_n$ for the recurrence found in 3.1:

$$\sum_{n \ge 1}\frac{c_n}{(n-1)!}t^{n-1}  = \sum_{n \ge 1}\frac{1}{(n-1)!} \bigg( \sum_{i + k = n} \binom{i + k - 1}{k}a_ib_k\bigg)t^{n-1}$$

We can separate the variables in the binomial coefficient.

$$\binom{i + k - 1}{k} = \frac{(i+k-1)!}{k!(i + k - 1 - k)!} = \frac{(n-1)!}{k!(i-1)!} $$

We then move the $(n-1)!$ term to the outer sum, cancelling the $\frac{1}{(n-1)!}$ term.

$$\sum_{n \ge 1}\frac{c_n}{(n-1)!}t^{n-1}  = \sum_{n \ge 1} \bigg( \sum_{i + k = n} \frac{a_ib_k}{(i-1)!k!}\bigg)t^{n-1}$$

We now separate the variables in this inner sum, then (appropriately) distribute the t power into the inner sum:

$$ = \sum_{n \ge 1} \bigg( \sum_{i + k = n} \frac{a_it^{i-1}}{(i-1)!} * \frac{b_kt^k}{k!}\bigg)$$

Where each term represents the convolution of $(a_{i+1})_{i \ge 0}$ and $(b_{k})_{k \ge 0}$. Thus $C'(t) = A'(t) \cdot B(t)$, and so:

$$C(z) = \int_{0}^{z} A'(t) \cdot B(t) dt$$

\section{Records}

\subsection{}

\subsection{}

\subsection{}

\subsection{}
Take the $m$-th derivative of $\mathcal P(x,z)$ with respect to z. Note this eliminates the first $m$ terms.

$$\frac{\partial^m \mathcal P(x,z)}{\partial z^m} = \sum_{n \ge m} \sum_{k = 1}^{n} \frac{r_{n,k}}{n!}\frac{n!}{(n-m)!}x^kz^{n-m}$$. 

In particular, the $m$-th term is $\sum_{k = 1}^{m}r_{m,k} x^k$ for all $z$. If $z = 0$, then this term is the only nonzero term remaining. Thus:

$$\sum_{k = 1}^{n}r_{m,k} x^k = \frac{\partial^m \mathcal P}{\partial z^m}(0,x) $$

Applying these operations to $\mathcal P(x,z) = (1-z)^{-x}$:

$$\frac{\partial}{\partial z^m} (1-z)^{-x}|_{z = 0} = (-1)^m(-x)(-x-1)(-x-2)....(-x - m + 1)(1-z)^{-x-m}|_{z = 0}$$
$$= (-1)^m(-1)^m(x)(x+1)(x+2)...(x + m -1)(1-z)^{-x-m}|_{z = 0}$$
$$= (x)(x+1)(x+2)...(x + m -1)$$

Which is our the result.

\subsection{}

Define the above expression as $F(x)$. From principles, the expected number of records in an $n$ size permutation is given by $F'(1)/F(1)$. $F(1)$ is straightforward to calculate:

$$F(1) = 1(1+1)(1 + 2)....(1 + m - 1) = m!$$

To find F'(1), Define a new function $G_j$ as:

$$G_j(x) = (x+m-1)(x+m-2)....(x+m-j), G_0(x) = 0$$

In particular:

$$G_m(x) = (x+m-1)(x+m-2)...(x+m-j) = F(x)$$ 
$$G_j(1) = m(m-1)...( (m-j)+1) = \frac{m!}{(m-j)!}$$

We can express the derivative of $G_m(x)$ as two parts via. the power rule:

$$G_k(x)|_{x = 1} = (x+m-k)' G_{k-1}(x) + (x+m-k)G'_{k-1}(x)|_{x = 1}$$
$$= G_{k-1}(1) + (m+1-k)*G'_{k-1}(x)|_{x = 1}$$

So we have a recurrence, with $R(k) = G_{k}(x)|_{x = 1}$:

$$R(k) = \frac{m!}{(m+1-k)!} + (m+1-k)R(k-1),   R(0) = 0$$

Evaluating the recursion at $m$ eventually gives:

$$F'(1) = R(m) = \sum_{k = 1}^{m} \frac{m!}{(m+1-k)!}*(m+1-(k+1))(m+1-(k+2))...(2)(1)$$
$$= \sum_{k = 1}^{m} \frac{m!}{(m-k+1)!}(m-k)! = m!\sum_{k = 1}^{m}\frac{1}{m+1-k} = m!\sum_{j = 1}^{m}\frac{1}{j}$$

And so the expected number of runs is:

$$E = F'(1)/F(1) = \frac{m!\sum_{j = 1}^{m}\frac{1}{j}}{m!} = \sum_{j = 1}^{m}\frac{1}{j} $$

I realized about halfway through this was complete overkill. 


\end{document}
